Translation.v
@@ -1,11 +1,9 @@
-Require Import Strings.String.
-Open Scope string_scope.
 Require Import List.
 Require Import Util.
 Require Import Lambda.
 Require Import TSO.
 Require Import SC.
-
+Require Import ZArith.
 
 Definition BUFFER_1A_CONST := 0.
 Definition BUFFER_1B_CONST := 1.
@@ -94,21 +92,46 @@ Definition translate_arrays (init : list (nat * (list nat))) (buf_size : nat) : 
   (1,nil) :: (* SPECIAL *)
   (1, 2 :: nil) :: nil. (* DONE_COUNTER *)
 
+
+Definition or (s : term) (t : term) := not (and (not s) (not t)).
+
+Definition equals (s : term) (t : term) := not (or (less_than s t) (less_than t s)).
+
+(* NEEDS TO BE CAPTURE-AVOIDING *)
+Definition seq (s : term) (t : term) := app (lam (shift_up 0 t)) s.
+
+Definition y_combinator := 
+  lam (app (lam (app (var 1) (app (var 0) (var 0)))) (lam (app (var 1) (app (var 0) (var 0)))) ).
+
+Definition while_fun := 
+  lam (lam (lam (case (var 1) (seq (var 0) (app (app (var 2) (var 1)) (var 0))) yunit))).
+
+Definition while_fics := app y_combinator while_fun.
+
+Definition while (s : term) (t : term) := app (app while_fics s) t.
+
+Notation "x == y" := (equals x y) (at level 60).
+
+Notation "c1 ;; c2" :=
+  (seq c1 c2) (at level 80, right associativity).
+Notation "'WHILE' b 'DO' c 'DONE'" :=
+  (while b c) (at level 80, right associativity).
+
 Definition read_code (thread : bool) (base : nat) (buf_size : nat) := 
   LOOP thread base ::= ZERO ;;
   FOUND thread base ::= ZERO ;;
   (WHILE !(LOOP thread base ) << (num buf_size) DO
-    (CASE (and ( (BUFFER_A thread base)[!(LOOP thread base)] == (& (first (var "pair"))) ) ( (BUFFER_B thread base)[!(LOOP thread base)] == (second (var "pair")) )) THEN
+    (CASE (and ( (BUFFER_A thread base)[!(LOOP thread base)] == (& (first (var 0))) ) ( (BUFFER_B thread base)[!(LOOP thread base)] == (second (var 0)) )) THEN
       RESULT thread base ::= (BUFFER_C thread base)[!(LOOP thread base)] ;;
       FOUND thread base ::= ONE
     ELSE
       yunit
     ESAC)
   DONE) ;;
-  CASE (!(FOUND thread base) == ONE) THEN !(RESULT thread base) ELSE (read (first (var "pair")) (second (var "pair"))) ESAC.
+  CASE (!(FOUND thread base) == ONE) THEN !(RESULT thread base) ELSE (read (first (var 0)) (second (var 0))) ESAC.
 
 Definition new_read (thread : bool) (base : nat) (buf_size : nat) (array : term) (offset : term)  : term :=
-  app (lam "pair" (read_code thread base buf_size)) (paire array offset).
+app (lam (read_code thread base buf_size)) (paire array offset).
 
 Definition flush (thread : bool) (base : nat) (buf_size : nat) : term :=
   CASE (!(SIZE thread base ) == ZERO) THEN yunit
@@ -121,13 +144,13 @@ Definition flush (thread : bool) (base : nat) (buf_size : nat) : term :=
 Definition write_code  (thread : bool) (base : nat) (buf_size : nat) :=
 CASE (!(SIZE thread base) == (num buf_size)) THEN (flush thread buf_size base) ELSE yunit ESAC ;;
   (REAR thread base) ::= modulo (plus (!(REAR thread base)) ONE) (num buf_size);;
-  (BUFFER_A thread base)[!(REAR thread base)] ::= (& (first (var "triple")));;
-  (BUFFER_B thread base)[!(REAR thread base)] ::= (first (second (var "triple")));;
-  (BUFFER_C thread base)[!(REAR thread base)] ::= (second (second (var "triple")));;
+  (BUFFER_A thread base)[!(REAR thread base)] ::= (& (first (var 0)));;
+  (BUFFER_B thread base)[!(REAR thread base)] ::= (first (second (var 0)));;
+  (BUFFER_C thread base)[!(REAR thread base)] ::= (second (second (var 0)));;
   (SIZE thread base) ::= plus (!(SIZE thread base)) ONE.
 
 Definition new_write (thread : bool) (base : nat) (buf_size : nat) (array : term) (offset : term) (value : term) : term :=
-  app (lam "triple" (write_code thread base buf_size)) (paire array (paire offset value)).
+app (lam (write_code thread base buf_size)) (paire array (paire offset value)).
 
 
 Definition flush_star (thread : bool) (base : nat) (buf_size : nat): term :=
@@ -145,42 +168,42 @@ Fixpoint translate (s : term) (thread : bool) (base : nat) (buf_size : nat) : te
     | fls => fls
     | yunit => yunit
     | var x => var x
-    | lam x e => lam x (seq (flush_star thread base buf_size) (translate e thread base buf_size))
+    | lam e => lam (seq (flush_star thread base buf_size) (translate e thread base buf_size))
     | app e1 e2 => 
       app (translate e1 thread base buf_size) (translate e2 thread base buf_size)
     | plus e1 e2 => 
       let x := translate e1 thread base buf_size in
       let y := translate e2 thread base buf_size in
-      app (lam "x" (seq (flush_star thread base buf_size) (var "x"))) (plus x y)
+      app (lam (seq (flush_star thread base buf_size) (var 0))) (plus x y)
     | minus e1 e2 =>
       let x := translate e1 thread base buf_size in
       let y := translate e2 thread base buf_size in
       let z := flush_star thread base buf_size in
-      app (lam "x" (seq (flush_star thread base buf_size) (var "x"))) (minus x y)
+      app (lam (seq (flush_star thread base buf_size) (var 0))) (minus x y)
     | modulo e1 e2 =>
       let x := translate e1 thread base buf_size in
       let y := translate e2 thread base buf_size in
       let z := flush_star thread base buf_size in
-      app (lam "x" (seq (flush_star thread base buf_size) (var "x"))) (modulo x y)
+      app (lam (seq (flush_star thread base buf_size) (var 0))) (modulo x y)
     | less_than e1 e2 =>
       let x := translate e1 thread base buf_size in
       let y := translate e2 thread base buf_size in
       let z := flush_star thread base buf_size in
-      app (lam "x" (seq (flush_star thread base buf_size) (var "x"))) (less_than x y)
+      app (lam (seq (flush_star thread base buf_size) (var 0))) (less_than x y)
     | and e1 e2 =>
       let x := translate e1 thread base buf_size in
       let y := translate e2 thread base buf_size in
       let z := flush_star thread base buf_size in
-      app (lam "x" (seq (flush_star thread base buf_size) (var "x"))) (and x y)
+      app (lam (seq (flush_star thread base buf_size) (var 0))) (and x y)
     | not e =>
       let x := translate e thread base buf_size in
-      app (lam "x" (seq (flush_star thread base buf_size) (var "x"))) (not x)
+      app (lam (seq (flush_star thread base buf_size) (var 0))) (not x)
     | reference e =>
       let x := translate e thread base buf_size in
-      app (lam "x" (seq (flush_star thread base buf_size) (var "x"))) (reference x)
+      app (lam (seq (flush_star thread base buf_size) (var 0))) (reference x)
     | cast e =>
       let x := translate e thread base buf_size in
-      app (lam "x" (seq (flush_star thread base buf_size) (var "x"))) (cast x)
+      app (lam (seq (flush_star thread base buf_size) (var 0))) (cast x)
     | case e1 e2 e3 =>
       let x := translate e1 thread base buf_size in
       let y := translate e2 thread base buf_size in
@@ -189,20 +212,20 @@ Fixpoint translate (s : term) (thread : bool) (base : nat) (buf_size : nat) : te
     | read e1 e2 =>
       let x := translate e1 thread base buf_size in
       let y := translate e2 thread base buf_size in
-      app (lam "x" (seq (flush_star thread base buf_size) (var "x"))) (new_read thread base buf_size x y)
+      app (lam (seq (flush_star thread base buf_size) (var 0))) (new_read thread base buf_size x y)
     | write e1 e2 e3 =>
       let x := translate e1 thread base buf_size in
       let y := translate e2 thread base buf_size in
       let z := translate e3 thread base buf_size in
-      app (lam "x" (seq (flush_star thread base buf_size) (var "x"))) (new_write thread base buf_size x y z)
+      app (lam (seq (flush_star thread base buf_size) (var 0))) (new_write thread base buf_size x y z)
     | paire e1 e2 =>
       paire (translate e1 thread base buf_size) (translate e2 thread base buf_size)
     | first e =>
       let x := translate e thread base buf_size in
-      app (lam "x" (seq (flush_star thread base buf_size) (var "x"))) (first x)
+      app (lam (seq (flush_star thread base buf_size) (var 0))) (first x)
     | second e =>
       let x := translate e thread base buf_size in
-      app (lam "x" (seq (flush_star thread base buf_size) (var "x"))) (second x)
+      app (lam (seq (flush_star thread base buf_size) (var 0))) (second x)
   end.
 
 Fact translate_var : forall x thread base buf_size, translate (var x) thread base buf_size = var x.
@@ -223,10 +246,10 @@ Proof. intros. simpl. reflexivity. Qed.
 Fact translate_yunit : forall thread base buf_size, translate yunit thread base buf_size = yunit.
 Proof. intros. simpl. reflexivity. Qed.
 
-Fact translate_lam : forall x e thread base buf_size, translate (lam x e) thread base buf_size = lam x (seq (flush_star thread base buf_size) (translate e thread base buf_size)).
+Fact translate_lam : forall e thread base buf_size, translate (lam e) thread base buf_size = lam (seq (flush_star thread base buf_size) (translate e thread base buf_size)).
 Proof. intros. simpl. reflexivity. Qed.
 
-Fact translate_plus : forall thread base buf_size e1 e2, translate (plus e1 e2) thread base buf_size = app (lam "x" (seq (flush_star thread base buf_size) (var "x"))) (plus (translate e1 thread base buf_size) (translate e2 thread base buf_size)).
+Fact translate_plus : forall thread base buf_size e1 e2, translate (plus e1 e2) thread base buf_size = app (lam (seq (flush_star thread base buf_size) (var 0))) (plus (translate e1 thread base buf_size) (translate e2 thread base buf_size)).
 Proof. intros. simpl. reflexivity. Qed.
 
 Fact translate_app : forall thread base buf_size e1 e2, translate (app e1 e2) thread base buf_size = app (translate e1 thread base buf_size) (translate e2 thread base buf_size).
@@ -235,126 +258,291 @@ Proof. intros. simpl. reflexivity. Qed.
 Fact translate_paire : forall thread base buf_size e1 e2, translate (paire e1 e2) thread base buf_size = paire (translate e1 thread base buf_size) (translate e2 thread base buf_size).
 Proof. intros. simpl. reflexivity. Qed.
 
-Fact translate_minus : forall thread base buf_size e1 e2, translate (minus e1 e2) thread base buf_size = app (lam "x" (seq (flush_star thread base buf_size) (var "x"))) (minus (translate e1 thread base buf_size) (translate e2 thread base buf_size)).
+Fact translate_minus : forall thread base buf_size e1 e2, translate (minus e1 e2) thread base buf_size = app (lam (seq (flush_star thread base buf_size) (var 0))) (minus (translate e1 thread base buf_size) (translate e2 thread base buf_size)).
 Proof. intros. simpl. reflexivity. Qed.
 
-Fact translate_modulo : forall thread base buf_size e1 e2, translate (modulo e1 e2) thread base buf_size = app (lam "x" (seq (flush_star thread base buf_size) (var "x"))) (modulo (translate e1 thread base buf_size) (translate e2 thread base buf_size)).
+Fact translate_modulo : forall thread base buf_size e1 e2, translate (modulo e1 e2) thread base buf_size = app (lam (seq (flush_star thread base buf_size) (var 0))) (modulo (translate e1 thread base buf_size) (translate e2 thread base buf_size)).
 Proof. intros. simpl. reflexivity. Qed.
 
-Fact translate_less_than : forall thread base buf_size e1 e2, translate (less_than e1 e2) thread base buf_size = app (lam "x" (seq (flush_star thread base buf_size) (var "x"))) (less_than (translate e1 thread base buf_size) (translate e2 thread base buf_size)).
+Fact translate_less_than : forall thread base buf_size e1 e2, translate (less_than e1 e2) thread base buf_size = app (lam (seq (flush_star thread base buf_size) (var 0))) (less_than (translate e1 thread base buf_size) (translate e2 thread base buf_size)).
 Proof. intros. simpl. reflexivity. Qed.
 
-Fact translate_and : forall thread base buf_size e1 e2, translate (and e1 e2) thread base buf_size = app (lam "x" (seq (flush_star thread base buf_size) (var "x"))) (and (translate e1 thread base buf_size) (translate e2 thread base buf_size)).
+Fact translate_and : forall thread base buf_size e1 e2, translate (and e1 e2) thread base buf_size = app (lam (seq (flush_star thread base buf_size) (var 0))) (and (translate e1 thread base buf_size) (translate e2 thread base buf_size)).
 Proof. intros. simpl. reflexivity. Qed.
 
-Fact translate_not : forall thread base buf_size e, translate (not e) thread base buf_size = app (lam "x" (seq (flush_star thread base buf_size) (var "x"))) (not (translate e thread base buf_size)).
+Fact translate_not : forall thread base buf_size e, translate (not e) thread base buf_size = app (lam (seq (flush_star thread base buf_size) (var 0))) (not (translate e thread base buf_size)).
 Proof. intros. simpl. reflexivity. Qed.
 
-Fact translate_cast : forall thread base buf_size e, translate (cast e) thread base buf_size = app (lam "x" (seq (flush_star thread base buf_size) (var "x"))) (cast (translate e thread base buf_size)).
+Fact translate_cast : forall thread base buf_size e, translate (cast e) thread base buf_size = app (lam (seq (flush_star thread base buf_size) (var 0))) (cast (translate e thread base buf_size)).
 Proof. intros. simpl. reflexivity. Qed.
 
-Fact translate_reference : forall thread base buf_size e, translate (reference e) thread base buf_size = app (lam "x" (seq (flush_star thread base buf_size) (var "x"))) (reference (translate e thread base buf_size)).
+Fact translate_reference : forall thread base buf_size e, translate (reference e) thread base buf_size = app (lam (seq (flush_star thread base buf_size) (var 0))) (reference (translate e thread base buf_size)).
 Proof. intros. simpl. reflexivity. Qed.
 
-Fact translate_first : forall thread base buf_size e, translate (first e) thread base buf_size = app (lam "x" (seq (flush_star thread base buf_size) (var "x"))) (first (translate e thread base buf_size)).
+Fact translate_first : forall thread base buf_size e, translate (first e) thread base buf_size = app (lam (seq (flush_star thread base buf_size) (var 0))) (first (translate e thread base buf_size)).
 Proof. intros. simpl. reflexivity. Qed.
 
-Fact translate_second : forall thread base buf_size e, translate (second e) thread base buf_size = app (lam "x" (seq (flush_star thread base buf_size) (var "x"))) (second (translate e thread base buf_size)).
+Fact translate_second : forall thread base buf_size e, translate (second e) thread base buf_size = app (lam (seq (flush_star thread base buf_size) (var 0))) (second (translate e thread base buf_size)).
 Proof. intros. simpl. reflexivity. Qed.
 
 Fact translate_case : forall thread base buf_size e1 e2 e3, translate (case e1 e2 e3) thread base buf_size = case (translate e1 thread base buf_size) (seq (flush_star thread base buf_size) (translate e2 thread base buf_size)) (seq (flush_star thread base buf_size) (translate e3 thread base buf_size)).
 Proof. intros. simpl. reflexivity. Qed.
 
-Fact translate_read : forall thread base buf_size e1 e2, translate (read e1 e2) thread base buf_size = app (lam "x" (seq (flush_star thread base buf_size) (var "x"))) (new_read thread base buf_size (translate e1 thread base buf_size)  (translate e2 thread base buf_size)).
+Fact translate_read : forall thread base buf_size e1 e2, translate (read e1 e2) thread base buf_size = app (lam (seq (flush_star thread base buf_size) (var 0))) (new_read thread base buf_size (translate e1 thread base buf_size)  (translate e2 thread base buf_size)).
 Proof. intros. simpl. reflexivity. Qed.
 
-Fact translate_write : forall thread base buf_size e1 e2 e3, translate (write e1 e2 e3) thread base buf_size = app (lam "x" (seq (flush_star thread base buf_size) (var "x"))) (new_write thread base buf_size (translate e1 thread base buf_size)  (translate e2 thread base buf_size) (translate e3 thread base buf_size)).
+Fact translate_write : forall thread base buf_size e1 e2 e3, translate (write e1 e2 e3) thread base buf_size = app (lam (seq (flush_star thread base buf_size) (var 0))) (new_write thread base buf_size (translate e1 thread base buf_size)  (translate e2 thread base buf_size) (translate e3 thread base buf_size)).
 Proof. intros. simpl. reflexivity. Qed.
+
+Fact subst_flush_star1 : forall x v thread base buf_size,
+  subst x v (flush_star thread base buf_size) = flush_star thread base buf_size.
+Proof. intros. simpl. assert (forall x, (x + 1 = S x)). intros. omega. repeat (rewrite H). destruct thread. simpl. auto. auto. Qed.
 
 Fact subst_flush_star : forall x v thread base buf_size,
-  subst x v (lam "x" (flush_star thread base buf_size;; var "x")) =
-  (lam "x" (flush_star thread base buf_size;; var "x")).
-Proof. intros. apply subst_idempotent. intros C. simpl in C. destruct thread; simpl in C; auto. Qed.
+  subst x v (lam (flush_star thread base buf_size;; var 0)) = (lam (flush_star thread base buf_size;; var 0)).
+Proof. intros. simpl. assert (forall x, (x + 1 = S x)). intros. omega. repeat (rewrite H). destruct thread. simpl. auto. auto. Qed.
 
+Fact new_read_subst_helper : forall x v thread base buf_size, subst x v (lam (read_code thread base buf_size)) = lam (read_code thread base buf_size).
+Proof. intros. rewrite subst_lam. unfold read_code. unfold seq. assert (forall x, (x + 1 = S x)). intros. omega. simpl. repeat (rewrite H). destruct thread. simpl. auto. auto. Qed.
 
 Fact new_read_subst : forall x v e1 e2 thread base buf_size,
   new_read thread base buf_size (subst x v e1) (subst x v e2) = subst x v (new_read thread base buf_size e1 e2).
-Proof. intros. unfold new_read. unfold read_code. rewrite subst_app. rewrite subst_paire. 
-assert (subst x v
-       (lam "pair"
-          (LOOP thread base [num 0]::= ZERO;;
-           FOUND thread base [num 0]::= ZERO;;
-           (WHILE (LOOP thread base [num 0]) << num buf_size
-            DO CASE and ((BUFFER_A thread base [LOOP thread base [num 0]]) == (& first (var "pair")))
-                      ((BUFFER_B thread base [LOOP thread base [num 0]]) == second (var "pair"))
-               THEN (RESULT thread base [num 0]::= BUFFER_C thread base) [LOOP thread base [num 0]];;
-                    FOUND thread base [num 0]::= ONE ELSE yunit ESAC DONE);;
-           CASE (FOUND thread base [num 0]) == ONE THEN RESULT thread base [num 0]
-           ELSE first (var "pair") [second (var "pair")] ESAC)) = lam "pair"
-       (LOOP thread base [num 0]::= ZERO;;
-        FOUND thread base [num 0]::= ZERO;;
-        (WHILE (LOOP thread base [num 0]) << num buf_size
-         DO CASE and ((BUFFER_A thread base [LOOP thread base [num 0]]) == (& first (var "pair")))
-                   ((BUFFER_B thread base [LOOP thread base [num 0]]) == second (var "pair"))
-            THEN (RESULT thread base [num 0]::= BUFFER_C thread base) [LOOP thread base [num 0]];;
-                 FOUND thread base [num 0]::= ONE ELSE yunit ESAC DONE);;
-        CASE (FOUND thread base [num 0]) == ONE THEN RESULT thread base [num 0]
-        ELSE first (var "pair") [second (var "pair")] ESAC)).
-{apply subst_idempotent. destruct thread; simpl; intros C; auto. } rewrite H. auto. Qed.
+Proof. intros. simpl. assert (forall x, (x + 1 = S x)). intros. omega. repeat (rewrite H). destruct thread. simpl. auto. auto. Qed.
 
 Fact new_write_subst : forall x v e1 e2 e3 thread base buf_size,
   new_write thread base buf_size (subst x v e1) (subst x v e2) (subst x v e3) = subst x v (new_write thread base buf_size e1 e2 e3).
-intros. unfold new_write. unfold write_code. rewrite subst_app. rewrite subst_paire. rewrite subst_paire.
-assert ((subst x v
-       (lam "triple"
-          ((CASE (SIZE thread base [num 0]) == num buf_size THEN flush thread buf_size base ELSE yunit
-            ESAC);;
-           REAR thread base [num 0]::= modulo (plus (REAR thread base [num 0]) ONE) (num buf_size);;
-           BUFFER_A thread base [REAR thread base [num 0]]::= (& first (var "triple"));;
-           BUFFER_B thread base [REAR thread base [num 0]]::= first (second (var "triple"));;
-           BUFFER_C thread base [REAR thread base [num 0]]::= second (second (var "triple"));;
-           SIZE thread base [num 0]::= plus (SIZE thread base [num 0]) ONE))) = (lam "triple"
-       ((CASE (SIZE thread base [num 0]) == num buf_size THEN flush thread buf_size base ELSE yunit ESAC);;
-        REAR thread base [num 0]::= modulo (plus (REAR thread base [num 0]) ONE) (num buf_size);;
-        BUFFER_A thread base [REAR thread base [num 0]]::= (& first (var "triple"));;
-        BUFFER_B thread base [REAR thread base [num 0]]::= first (second (var "triple"));;
-        BUFFER_C thread base [REAR thread base [num 0]]::= second (second (var "triple"));;
-        SIZE thread base [num 0]::= plus (SIZE thread base [num 0]) ONE))).
-{ apply subst_idempotent. destruct thread; intros C; auto. } rewrite H. auto. Qed.
+Proof. intros. simpl. assert (forall x, (x + 1 = S x)). intros. omega. repeat (rewrite H). destruct thread. simpl. auto. auto. Qed.
+
+Fixpoint shift_up_n_c n c e  :=
+  match n with
+    | 0 => e
+    | S n => shift_up_n_c n c (shift_up c e)
+  end.
+
+Definition shift_up_n n e := shift_up_n_c n 0 e.
+
+Fact shift_up_n_c_array : forall n c k, shift_up_n_c n c (array k) = array k.
+Proof. intros. generalize dependent k. generalize dependent c. induction n ; intros.
+  + simpl. auto.
+  + simpl. rewrite IHn. auto. Qed.
+
+Fact shift_up_n_c_num : forall n c k, shift_up_n_c n c (num k) = num k.
+Proof. intros. generalize dependent k. generalize dependent c. induction n ; intros.
+  + simpl. auto.
+  + simpl. rewrite IHn. auto. Qed.
+
+Fact shift_up_n_c_tru : forall n c, shift_up_n_c n c tru = tru.
+Proof. intros. generalize dependent c. induction n ; intros.
+  + simpl. auto.
+  + simpl. rewrite IHn. auto. Qed.
+
+Fact shift_up_n_c_fls : forall n c, shift_up_n_c n c fls = fls.
+Proof. intros. generalize dependent c. induction n ; intros.
+  + simpl. auto.
+  + simpl. rewrite IHn. auto. Qed.
+
+Fact shift_up_n_c_yunit : forall n c, shift_up_n_c n c yunit = yunit.
+Proof. intros. generalize dependent c. induction n ; intros.
+  + simpl. auto.
+  + simpl. rewrite IHn. auto. Qed.
+
+Fact shift_up_n_c_plus : forall n c e1 e2, shift_up_n_c n c (plus e1 e2) = plus (shift_up_n_c n c e1) (shift_up_n_c n c e2).
+Proof. intros. generalize dependent c. generalize dependent e1. generalize dependent e2. induction n ; intros.
+  + simpl. auto.
+  + simpl. rewrite IHn. auto. Qed.
+
+Fact shift_up_n_c_minus : forall n c e1 e2, shift_up_n_c n c (minus e1 e2) = minus (shift_up_n_c n c e1) (shift_up_n_c n c e2).
+Proof. intros. generalize dependent c. generalize dependent e1. generalize dependent e2. induction n ; intros.
+  + simpl. auto.
+  + simpl. rewrite IHn. auto. Qed.
+
+Fact shift_up_n_c_modulo : forall n c e1 e2, shift_up_n_c n c (modulo e1 e2) = modulo (shift_up_n_c n c e1) (shift_up_n_c n c e2).
+Proof. intros. generalize dependent c. generalize dependent e1. generalize dependent e2. induction n ; intros.
+  + simpl. auto.
+  + simpl. rewrite IHn. auto. Qed.
+
+Fact shift_up_n_c_less_than : forall n c e1 e2, shift_up_n_c n c (less_than e1 e2) = less_than (shift_up_n_c n c e1) (shift_up_n_c n c e2).
+Proof. intros. generalize dependent c. generalize dependent e1. generalize dependent e2. induction n ; intros.
+  + simpl. auto.
+  + simpl. rewrite IHn. auto. Qed.
+
+Fact shift_up_n_c_and : forall n c e1 e2, shift_up_n_c n c (and e1 e2) = and (shift_up_n_c n c e1) (shift_up_n_c n c e2).
+Proof. intros. generalize dependent c. generalize dependent e1. generalize dependent e2. induction n ; intros.
+  + simpl. auto.
+  + simpl. rewrite IHn. auto. Qed.
+
+Fact shift_up_n_c_read : forall n c e1 e2, shift_up_n_c n c (read e1 e2) = read (shift_up_n_c n c e1) (shift_up_n_c n c e2).
+Proof. intros. generalize dependent c. generalize dependent e1. generalize dependent e2. induction n ; intros.
+  + simpl. auto.
+  + simpl. rewrite IHn. auto. Qed.
+
+Fact shift_up_n_c_app : forall n c e1 e2, shift_up_n_c n c (app e1 e2) = app (shift_up_n_c n c e1) (shift_up_n_c n c e2).
+Proof. intros. generalize dependent c. generalize dependent e1. generalize dependent e2. induction n ; intros.
+  + simpl. auto.
+  + simpl. rewrite IHn. auto. Qed.
+
+Fact shift_up_n_c_write : forall n c e1 e2 e3, shift_up_n_c n c (write e1 e2 e3) = write (shift_up_n_c n c e1) (shift_up_n_c n c e2) (shift_up_n_c n c e3).
+Proof. intros. generalize dependent c. generalize dependent e1. generalize dependent e2. generalize dependent e3. induction n ; intros.
+  + simpl. auto.
+  + simpl. rewrite IHn. auto. Qed.
+
+Fact shift_up_n_c_case : forall n c e1 e2 e3, shift_up_n_c n c (case e1 e2 e3) = case (shift_up_n_c n c e1) (shift_up_n_c n c e2) (shift_up_n_c n c e3).
+Proof. intros. generalize dependent c. generalize dependent e1. generalize dependent e2. generalize dependent e3. induction n ; intros.
+  + simpl. auto.
+  + simpl. rewrite IHn. auto. Qed.
+
+Fact shift_up_n_c_paire : forall n c e1 e2, shift_up_n_c n c (paire e1 e2) = paire (shift_up_n_c n c e1) (shift_up_n_c n c e2).
+Proof. intros. generalize dependent c. generalize dependent e1. generalize dependent e2. induction n ; intros.
+  + simpl. auto.
+  + simpl. rewrite IHn. auto. Qed.
+
+Fact shift_up_n_c_cast : forall n c e, shift_up_n_c n c (cast e) = cast (shift_up_n_c n c e).
+Proof. intros. generalize dependent c. generalize dependent e. induction n ; intros.
+  + simpl. auto.
+  + simpl. rewrite IHn. auto. Qed.
+
+Fact shift_up_n_c_not : forall n c e, shift_up_n_c n c (not e) = not (shift_up_n_c n c e).
+Proof. intros. generalize dependent c. generalize dependent e. induction n ; intros.
+  + simpl. auto.
+  + simpl. rewrite IHn. auto. Qed.
+
+Fact shift_up_n_c_reference : forall n c e, shift_up_n_c n c (reference e) = reference (shift_up_n_c n c e).
+Proof. intros. generalize dependent c. generalize dependent e. induction n ; intros.
+  + simpl. auto.
+  + simpl. rewrite IHn. auto. Qed.
+
+Fact shift_up_n_c_first : forall n c e, shift_up_n_c n c (first e) = first (shift_up_n_c n c e).
+Proof. intros. generalize dependent c. generalize dependent e. induction n ; intros.
+  + simpl. auto.
+  + simpl. rewrite IHn. auto. Qed.
+
+Fact shift_up_n_c_second : forall n c e, shift_up_n_c n c (second e) = second (shift_up_n_c n c e).
+Proof. intros. generalize dependent c. generalize dependent e. induction n ; intros.
+  + simpl. auto.
+  + simpl. rewrite IHn. auto. Qed.
 
 
-Fact seq_flush_subst : forall x v thread base buf_size e, subst x v (flush_star thread base buf_size;; e) =  (flush_star thread base buf_size;; (subst x v e)).
-Proof. intros. unfold flush_star. unfold flush. unfold seq. rewrite subst_app. rewrite subst_app. rewrite subst_app. rewrite subst_lam. rewrite subst_lam. rewrite subst_app. rewrite subst_lam. rewrite subst_lam. rewrite subst_var. assert (subst x v (SPECIAL base [num 0]::= ONE) = (SPECIAL base [num 0]::= ONE)). apply subst_idempotent. intros C. simpl in C. auto. rewrite H. assert (subst x v
-             (WHILE and ((SPECIAL base [num 0]) == ONE) (not ((SIZE thread base [num 0]) == ZERO))
-              DO CASE (SIZE thread base [num 0]) == ZERO THEN yunit
-                 ELSE app
-                        (app (lam "x" (lam "y" (var "y")))
-                           (cast (BUFFER_A thread base [FRONT thread base [num 0]])
-                            [BUFFER_B thread base [FRONT thread base [num 0]]]
-                            ::= (BUFFER_C thread base [FRONT thread base [num 0]])))
-                        (app
-                           (app (lam "x" (lam "y" (var "y")))
-                              (FRONT thread base [num 0]
-                               ::= modulo (plus (FRONT thread base [num 0]) ONE) (num buf_size)))
-                           (SIZE thread base [num 0]::= minus (SIZE thread base [num 0]) ONE)) ESAC DONE) =
-             (WHILE and ((SPECIAL base [num 0]) == ONE) (not ((SIZE thread base [num 0]) == ZERO))
-              DO CASE (SIZE thread base [num 0]) == ZERO THEN yunit
-                 ELSE app
-                        (app (lam "x" (lam "y" (var "y")))
-                           (cast (BUFFER_A thread base [FRONT thread base [num 0]])
-                            [BUFFER_B thread base [FRONT thread base [num 0]]]
-                            ::= (BUFFER_C thread base [FRONT thread base [num 0]])))
-                        (app
-                           (app (lam "x" (lam "y" (var "y")))
-                              (FRONT thread base [num 0]
-                               ::= modulo (plus (FRONT thread base [num 0]) ONE) (num buf_size)))
-                           (SIZE thread base [num 0]::= minus (SIZE thread base [num 0]) ONE)) ESAC DONE)). apply subst_idempotent. simpl. destruct thread; simpl; auto. rewrite H0. clear H0. destruct (string_dec x "x"); destruct (string_dec x "y"); auto.
+Fact shift_up_n_c_lam : forall n c e, shift_up_n_c n c (lam e) = lam (shift_up_n_c n (c+1) e).
+Proof. intros. generalize dependent e. generalize dependent c. induction n ; intros.
+  + simpl. auto.
+  + simpl. rewrite IHn. auto. Qed.
+
+Fact shift_up_n_c_var1 : forall n c k, k < c -> shift_up_n_c n c (var k) = var k.
+Proof. intros. generalize dependent k. generalize dependent c. induction n ; intros.
+  + simpl. auto.
+  + simpl. destruct (k <? c) eqn:ORIG.
+    ++ apply Nat.ltb_lt in ORIG. apply IHn. auto.
+    ++ apply Nat.ltb_lt in H. rewrite H in ORIG. inversion ORIG. Qed.
+
+Fact shift_up_n_c_var2 : forall n c k, k >= c -> shift_up_n_c n c (var k) = var (n+k).
+Proof. intros. generalize dependent k. generalize dependent c. induction n ; intros.
+  + simpl. auto.
+  + simpl. destruct (k <? c) eqn:ORIG.
+    ++ apply Nat.ltb_lt in ORIG. omega.
+    ++ rewrite IHn. assert (n+(k+1) = S(n+k)). omega. rewrite H0. auto. omega. Qed.
+
+
+Fact shift_up_n_eq : forall n c e, shift_up_n_c (n + 1) c e = shift_up (n+c) (shift_up_n_c n c e).
+Proof. intros. generalize dependent c. generalize dependent n. induction e ; intros.
+  + rewrite shift_up_n_c_array. rewrite shift_up_n_c_array. simpl. auto.
+  + rewrite shift_up_n_c_num. rewrite shift_up_n_c_num. simpl. auto.
+  + rewrite shift_up_n_c_plus. rewrite shift_up_n_c_plus. rewrite IHe1. rewrite IHe2. simpl. auto.
+  + rewrite shift_up_n_c_minus. rewrite shift_up_n_c_minus. rewrite IHe1. rewrite IHe2. simpl. auto.
+  + rewrite shift_up_n_c_modulo. rewrite shift_up_n_c_modulo. rewrite IHe1. rewrite IHe2. simpl. auto.
+  + rewrite shift_up_n_c_tru. rewrite shift_up_n_c_tru. simpl. auto.
+  + rewrite shift_up_n_c_fls. rewrite shift_up_n_c_fls. simpl. auto.
+  + rewrite shift_up_n_c_less_than. rewrite shift_up_n_c_less_than. rewrite IHe1. rewrite IHe2. simpl. auto. 
+  + rewrite shift_up_n_c_not. rewrite shift_up_n_c_not. rewrite IHe. simpl. auto.
+  + rewrite shift_up_n_c_and. rewrite shift_up_n_c_and. rewrite IHe1. rewrite IHe2. simpl. auto.
+  + rewrite shift_up_n_c_yunit. rewrite shift_up_n_c_yunit. simpl. auto.
+  + rewrite shift_up_n_c_read. rewrite shift_up_n_c_read. rewrite IHe1. rewrite IHe2. simpl. auto.
+  + rewrite shift_up_n_c_write. rewrite shift_up_n_c_write. rewrite IHe1. rewrite IHe2. rewrite IHe3. simpl. auto.
+  + rewrite shift_up_n_c_reference. rewrite shift_up_n_c_reference. rewrite IHe. simpl. auto.
+  + rewrite shift_up_n_c_cast. rewrite shift_up_n_c_cast. rewrite IHe. simpl. auto.
+  + rewrite shift_up_n_c_case. rewrite shift_up_n_c_case. rewrite IHe1. rewrite IHe2. rewrite IHe3. simpl. auto.
+  + destruct (n <? c) eqn:ORIG. apply Nat.ltb_lt in ORIG. rewrite shift_up_n_c_var1. rewrite shift_up_n_c_var1. simpl. destruct (n <? n0 + c) eqn:ORIG1. apply Nat.ltb_lt in ORIG1. auto. assert (n < n0 + c -> False). intros. apply Nat.ltb_lt in H. rewrite H in ORIG1. inversion ORIG1. contradiction H. omega. auto. auto. assert (n <  c -> False). intros. apply Nat.ltb_lt in H. rewrite ORIG in H. inversion H. assert (n >= c). omega. rewrite shift_up_n_c_var2. rewrite shift_up_n_c_var2. simpl. destruct (n0 + n <? n0 + c) eqn:ORIG1. rewrite Nat.ltb_lt in ORIG1. omega. assert (n0+1+n=n0+n+1). omega. rewrite H1. auto. auto. auto.
+  + rewrite shift_up_n_c_app. rewrite shift_up_n_c_app. rewrite IHe1. rewrite IHe2. simpl. auto.
+  + rewrite shift_up_n_c_lam. rewrite shift_up_n_c_lam. assert (n+1=S n). omega. repeat (rewrite H in *). simpl. assert (shift_up_n_c (n + 1) (c+1) e =
+shift_up (n + (c + 1)) (shift_up_n_c n (c + 1) e)). apply IHe. assert (n+c+1=n+(c+1)). omega. rewrite H1 in *. rewrite <- H0. assert (n+1=S n). omega. rewrite H2 in *. simpl. auto.
+  + rewrite shift_up_n_c_paire. rewrite shift_up_n_c_paire. rewrite IHe1. rewrite IHe2. simpl. auto.
+  + rewrite shift_up_n_c_first. rewrite shift_up_n_c_first. rewrite IHe. simpl. auto.
+  + rewrite shift_up_n_c_second. rewrite shift_up_n_c_second. rewrite IHe. simpl. auto.
 Qed.
 
+Fact foo : forall n e, shift_up_n_c (S n) 0 e = shift_up 0 (shift_up_n_c n 0 e).
+Proof. intros. generalize dependent e. induction n ; intros ; simpl.
+  + auto.
+  + rewrite <- IHn. simpl. auto. Qed.
+
+Fact blah : forall x v e c, subst (x + (c+1)) (shift_up_n (c+1) v) (shift_up c e) =
+shift_up c (subst (x + c) (shift_up_n c v) e).
+Proof. intros. generalize dependent x. generalize dependent v. generalize dependent c. induction e ; intros ; simpl ; try auto ; try (rewrite IHe1 ; rewrite IHe2 ; auto); try (rewrite IHe3 ; auto) ; try (rewrite IHe ; auto). destruct (n =? x + c) eqn:ORIG. apply beq_nat_true in ORIG. subst. destruct (x + c <? c) eqn:ORIG. rewrite Nat.ltb_lt in ORIG. omega. simpl. destruct (x + c + 1 =? x + (c + 1)) eqn:ORIG1. apply beq_nat_true in ORIG1. unfold shift_up_n. rewrite shift_up_n_eq. assert (c+0=c). omega. rewrite H. auto. apply beq_nat_false in ORIG1. contradiction ORIG1. omega. destruct (n <? c) eqn:ORIG1. apply Nat.ltb_lt in ORIG1. simpl. destruct ( n =? x + (c + 1)) eqn:ORIG2. apply beq_nat_true in ORIG2. subst. omega. destruct (n <? c) eqn:ORIG3. auto. assert ((n <? c) = true -> False). intros. rewrite ORIG3 in H. inversion H. assert ((n <? c) = true). apply Nat.ltb_lt. auto. apply H in H0. contradiction. simpl. destruct (n + 1 =? x + (c + 1)) eqn:ORIG2. apply beq_nat_true in ORIG2. assert (n=x+c). omega. subst. apply beq_nat_false in ORIG. contradiction ORIG. auto. destruct (n <? c) eqn:ORIG3. inversion ORIG1. auto. unfold shift_up_n in *. rewrite <- foo. rewrite <- foo. assert (x+(c+1)+1=x+((c+1)+1)). omega. rewrite H. clear H. assert (S (c+1) = (c+1)+1). omega. rewrite H. clear H. rewrite IHe. assert (x+(c+1)=x+c+1). omega. rewrite H. auto. clear H. assert (c+1=S c). omega. rewrite H. auto. Qed.
+
+
+Fact helper : forall x v e, subst (x + 1) (shift_up 0 v) (shift_up 0 e) = shift_up 0 (subst x v e).
+Proof. intros. intros. generalize dependent x. generalize dependent v. induction e ; intros ; simpl ; auto ; try (rewrite IHe1 ; rewrite IHe2 ; auto) ; try (rewrite IHe3 ; auto) ; try (rewrite IHe ; auto).
+  + destruct (n + 1 =? x + 1) eqn:ORIG.
+    ++ apply beq_nat_true in ORIG. assert (n=x). omega. subst. destruct (x =? x) eqn:ORIG1. auto. apply beq_nat_false in ORIG1. contradiction ORIG1. auto.
+    ++ apply beq_nat_false in ORIG. assert (n <> x). omega. destruct (n =? x) eqn:ORIG1. apply beq_nat_true in ORIG1. subst. contradiction H. auto. simpl. auto.
+  + assert (shift_up 0 (shift_up 0 v) = shift_up_n_c (1+1) 0 v). rewrite foo. rewrite foo. simpl. auto. rewrite H. clear H. assert (shift_up_n_c (1 + 1) 0 v = shift_up_n (1+1) v). unfold shift_up_n. auto. rewrite H. clear H. assert (x+1+1=x+(1+1)). omega. rewrite H. rewrite blah.
+simpl. unfold shift_up_n. simpl. auto. Qed.
+
+Fact seq_subst : forall x v e e', subst x v (e;;e') = ((subst x v e) ;; (subst x v e')).
+Proof. intros. unfold seq. rewrite subst_app. rewrite subst_lam. rewrite helper. auto. Qed.
+
+Fact shift_up_flush_star1 : forall c thread base buf_size,
+  shift_up c(flush_star thread base buf_size) = flush_star thread base buf_size.
+Proof. intros. simpl. assert (forall x, (x + 1 = S x)). intros. omega. repeat (rewrite H). destruct thread. simpl. auto. auto. Qed.
+
+Fact shift_up_new_read_star1 : forall c thread base buf_size e1 e2,
+  shift_up c (new_read thread base buf_size e1 e2) = new_read thread base buf_size  (shift_up c e1) (shift_up c e2).
+Proof. intros. unfold new_read. unfold read_code. simpl. assert (forall x, (x + 1 = S x)). intros. omega. repeat (rewrite H). destruct thread. simpl. auto. auto. Qed.
+
+Fact shift_up_new_write_star1 : forall c thread base buf_size e1 e2 e3,
+  shift_up c (new_write thread base buf_size e1 e2 e3) = new_write thread base buf_size  (shift_up c e1) (shift_up c e2) (shift_up c e3).
+Proof. intros. unfold new_write. unfold write_code. simpl. assert (forall x, (x + 1 = S x)). intros. omega. repeat (rewrite H). destruct thread. simpl. auto. auto. Qed.
+
+Fact foo1 : forall c k e, shift_up (c + k + 1) (shift_up k e) = shift_up k (shift_up (c + k) e).
+Proof. intros. generalize dependent c. generalize dependent k. induction e ; intros ; simpl ; auto ; try (rewrite IHe1 ; rewrite IHe2 ; auto) ; try (rewrite IHe3 ; auto) ; try (rewrite IHe ; auto). 
+  + destruct (n <? k) eqn:ORIG.
+    ++ assert (COPY:=ORIG). apply Nat.ltb_lt in ORIG. assert (n  <? c + k = true). apply Nat.ltb_lt. omega. rewrite H. apply Nat.ltb_lt in H. simpl. rewrite COPY. assert (n <? c+k+1 = true). apply Nat.ltb_lt. omega. rewrite H0. auto.
+    ++ simpl. destruct (n + 1 <? c + k + 1) eqn:ORIG1. apply Nat.ltb_lt in ORIG1. assert (n <? c+k = true). apply Nat.ltb_lt. omega. rewrite H. simpl. destruct (n <? k) eqn:ORIG2. inversion ORIG. auto. assert (n + 1 <? c + k + 1 = true -> False). intros. rewrite ORIG1 in H. inversion H. destruct (n <? c + k) eqn:ORIG2. contradiction H. apply Nat.ltb_lt. apply Nat.ltb_lt in ORIG2. omega. simpl. destruct (n + 1 <? k) eqn:ORIG3. apply Nat.ltb_lt in ORIG3. assert (n<k -> False). intros. apply Nat.ltb_lt in H0. rewrite ORIG in H0. inversion H0. clear ORIG1. contradiction H0. omega. auto.
+  + assert (c+k+1+1=c+(k+1)+1). omega. rewrite H. rewrite IHe. assert (c+(k+1)=c+k+1). omega. rewrite H0. auto. Qed.
+
+Fact shift_up_seq : forall c e1 e2 , shift_up c (e1;;e2) = ((shift_up c e1);;(shift_up c e2)).
+Proof. intros. unfold seq. rewrite shift_up_app. rewrite shift_up_lam. assert (shift_up (c + 1) (shift_up 0 e2) = shift_up 0 (shift_up c e2)). assert (c+0+1=c+1). omega. rewrite <- H. rewrite foo1. assert (c+0=c). omega. rewrite H0. auto. rewrite H. auto. Qed.
+
+Fact shift_commutes_with_translate : forall c e thread base buf_size, translate (shift_up c e) thread base buf_size = shift_up c (translate e thread base buf_size).
+Proof. intros. generalize dependent c; induction e ; intros.
+  + simpl. auto.
+  + simpl. auto.
+  + rewrite shift_up_plus. rewrite translate_plus. rewrite translate_plus. rewrite shift_up_app. rewrite shift_up_plus. rewrite shift_up_lam. rewrite shift_up_seq. rewrite shift_up_flush_star1. rewrite IHe1. rewrite IHe2. destruct c; simpl ; auto.
+  + rewrite shift_up_minus. rewrite translate_minus. rewrite translate_minus. rewrite shift_up_app. rewrite shift_up_minus. rewrite shift_up_lam. rewrite shift_up_seq. rewrite shift_up_flush_star1. rewrite IHe1. rewrite IHe2. simpl. destruct c; simpl ; auto.
+  + rewrite shift_up_modulo. rewrite translate_modulo. rewrite translate_modulo. rewrite shift_up_app. rewrite shift_up_modulo. rewrite shift_up_lam. rewrite shift_up_seq. rewrite shift_up_flush_star1. rewrite IHe1. rewrite IHe2. destruct c; simpl ; auto.
+  + simpl. auto.
+  + simpl. auto.
+  + rewrite shift_up_less_than. rewrite translate_less_than. rewrite translate_less_than. rewrite shift_up_app. rewrite shift_up_less_than. rewrite shift_up_lam. rewrite shift_up_seq. rewrite shift_up_flush_star1. rewrite IHe1. rewrite IHe2. destruct c; simpl ; auto.
+  + rewrite shift_up_not. rewrite translate_not. rewrite translate_not. rewrite shift_up_app. rewrite shift_up_not. rewrite shift_up_lam. rewrite shift_up_seq. rewrite shift_up_flush_star1. rewrite IHe. destruct c; simpl ; auto.
+  + rewrite shift_up_and. rewrite translate_and. rewrite translate_and. rewrite shift_up_app. rewrite shift_up_and. rewrite shift_up_lam. rewrite shift_up_seq. rewrite shift_up_flush_star1. rewrite IHe1. rewrite IHe2. simpl. destruct c; simpl ; auto.
+  + simpl. auto.
+  + rewrite shift_up_read. rewrite translate_read. rewrite translate_read. rewrite shift_up_app. rewrite IHe1. rewrite IHe2. rewrite shift_up_new_read_star1. rewrite shift_up_lam. rewrite shift_up_seq. rewrite shift_up_flush_star1. destruct c; simpl ; auto.
+  + rewrite shift_up_write. rewrite translate_write. rewrite translate_write. rewrite shift_up_app. rewrite IHe1. rewrite IHe2. rewrite IHe3. rewrite shift_up_new_write_star1. rewrite shift_up_lam. rewrite shift_up_seq. rewrite shift_up_flush_star1. simpl (shift_up (0 + 1) (var 0)). destruct c; simpl ; auto.
+  + rewrite shift_up_reference. rewrite translate_reference. rewrite translate_reference. rewrite shift_up_app. rewrite shift_up_reference. rewrite shift_up_lam. rewrite shift_up_seq. rewrite shift_up_flush_star1. rewrite IHe. destruct c; simpl ; auto.
+  + rewrite shift_up_cast. rewrite translate_cast. rewrite translate_cast. rewrite shift_up_app. rewrite shift_up_cast. rewrite shift_up_lam. rewrite shift_up_seq. rewrite shift_up_flush_star1. rewrite IHe. destruct c; simpl ; auto.
+  + rewrite shift_up_case. rewrite translate_case. rewrite translate_case. rewrite shift_up_case. rewrite shift_up_seq. rewrite shift_up_flush_star1. rewrite shift_up_seq. rewrite shift_up_flush_star1. rewrite IHe1. rewrite IHe2. rewrite IHe3. destruct c; simpl ; auto.
+  + simpl. destruct (n <? c); simpl ; auto.
+  + rewrite shift_up_app. rewrite translate_app. rewrite translate_app. rewrite shift_up_app. rewrite IHe1. rewrite IHe2. destruct c; simpl ; auto.
+  + rewrite shift_up_lam. rewrite translate_lam. rewrite translate_lam. rewrite shift_up_lam. rewrite shift_up_seq. rewrite shift_up_flush_star1. rewrite IHe. auto.
+  + rewrite shift_up_paire. rewrite translate_paire. rewrite translate_paire. rewrite shift_up_paire. rewrite IHe1. rewrite IHe2. destruct c; simpl ; auto.
+  + rewrite shift_up_first. rewrite translate_first. rewrite translate_first. rewrite shift_up_app. rewrite shift_up_first. rewrite shift_up_lam. rewrite shift_up_seq. rewrite shift_up_flush_star1. rewrite IHe. destruct c; simpl ; auto.
+  + rewrite shift_up_second. rewrite translate_second. rewrite translate_second. rewrite shift_up_app. rewrite shift_up_second. rewrite shift_up_lam. rewrite shift_up_seq. rewrite shift_up_flush_star1. rewrite IHe. destruct c; simpl ; auto. Qed.
+
+Fact seq_flush_subst : forall x v thread base buf_size e, subst x v (flush_star thread base buf_size;; e) =  (flush_star thread base buf_size;; (subst x v e)).
+Proof. intros. rewrite seq_subst. rewrite subst_flush_star1. auto. Qed.
 
 Fact trans_subst : forall x v e thread base buf_size, 
   translate (subst x v e) thread base buf_size = subst x (translate v thread base buf_size) (translate e thread base buf_size).
-Proof. intros. induction e.
+Proof. intros. generalize dependent v. generalize dependent x. induction e ; intros.
   + rewrite subst_array. simpl. reflexivity.
   + rewrite subst_num. simpl. reflexivity.
   + rewrite subst_plus. rewrite translate_plus. rewrite translate_plus. rewrite subst_app. rewrite subst_plus. rewrite IHe1. rewrite IHe2. rewrite subst_flush_star. reflexivity.
@@ -371,14 +559,9 @@ Proof. intros. induction e.
   + rewrite subst_reference. rewrite translate_reference. rewrite translate_reference. rewrite subst_app. rewrite subst_reference. rewrite IHe. rewrite subst_flush_star. reflexivity.
   + rewrite subst_cast. rewrite translate_cast. rewrite translate_cast. rewrite subst_app. rewrite subst_cast. rewrite IHe. rewrite subst_flush_star. reflexivity.
   + rewrite subst_case. rewrite translate_case. rewrite translate_case. rewrite subst_case. rewrite IHe1. rewrite IHe2. rewrite IHe3. rewrite seq_flush_subst. rewrite seq_flush_subst. auto.
-  + rewrite subst_var. rewrite translate_var. rewrite subst_var. destruct (string_dec x s).
-    ++ reflexivity.
-    ++ rewrite translate_var. reflexivity.
-  + rewrite subst_app. rewrite translate_app. rewrite translate_app. rewrite subst_app. rewrite IHe1. rewrite IHe2. reflexivity.
-  + rewrite subst_lam. rewrite translate_lam. rewrite translate_lam. rewrite subst_lam.
-destruct (string_dec x s).
-    ++ subst. reflexivity.
-    ++ rewrite IHe. rewrite seq_flush_subst. auto.
+  + rewrite subst_var. simpl. destruct (n =? x). auto. simpl. auto.
+  + rewrite subst_app. rewrite translate_app. rewrite IHe1. rewrite IHe2. reflexivity.
+  + rewrite subst_lam. rewrite translate_lam. rewrite translate_lam. rewrite subst_lam. rewrite seq_subst. rewrite subst_flush_star1. rewrite IHe. rewrite shift_commutes_with_translate. auto.
   + rewrite subst_paire. rewrite translate_paire. rewrite translate_paire. rewrite subst_paire. rewrite IHe1. rewrite IHe2. reflexivity.
   + rewrite subst_first. rewrite translate_first. rewrite translate_first. rewrite subst_app. rewrite subst_first. rewrite IHe. rewrite subst_flush_star. reflexivity.
   + rewrite subst_second. rewrite translate_second. rewrite translate_second. rewrite subst_app. rewrite subst_second. rewrite IHe. rewrite subst_flush_star. reflexivity.
@@ -394,7 +577,6 @@ Proof. intros. induction H; simpl.
   + apply value_fls.
   + apply value_lam.
   + apply value_paire. auto. auto. Qed.
-
 
 
 Fact translation_of_context_steps : forall e e' b B buf_size f m' m'0 l l' thread E u v u' v',
@@ -414,7 +596,7 @@ Proof. intros. generalize dependent l. generalize dependent l'. generalize depen
     ++ intros. destruct (thread_equals t0 thread) eqn:ORIG.
        +++ rewrite Heqthreads'. rewrite ORIG. rewrite H2. rewrite ORIG. auto.
        +++ rewrite Heqthreads'. rewrite ORIG. rewrite H2. rewrite ORIG. auto.
-  + destruct s. destruct e0. destruct H4. subst x. rewrite translate_app in *. rewrite translate_lam in *. apply steps_app_right with (threads:=threads) (threads':=threads') (thread:=thread) (x:=x0) (e2:=flush_star b B buf_size;; translate x1 b B buf_size).
+  + destruct s. destruct e0. subst x. rewrite translate_app in *. rewrite translate_lam in *. apply steps_app_right with (threads:=threads) (threads':=threads') (thread:=thread) (e2:=flush_star b B buf_size;; translate x0 b B buf_size).
     ++ apply IHE with (u:=u) (v:=v). rewrite Heqthreads'. auto. auto. rewrite Heqthreads. auto. auto. auto.
     ++ intros. destruct (thread_equals t thread) eqn:ORIG.
        +++ rewrite Heqthreads. rewrite ORIG. rewrite H1. rewrite ORIG. auto.
@@ -422,7 +604,7 @@ Proof. intros. generalize dependent l. generalize dependent l'. generalize depen
     ++ intros. destruct (thread_equals t thread) eqn:ORIG.
        +++ rewrite Heqthreads'. rewrite ORIG. rewrite H2. rewrite ORIG. auto.
        +++ rewrite Heqthreads'. rewrite ORIG. rewrite H2. rewrite ORIG. auto.
-  + remember (fun t0 => if thread_equals t0 thread then plus (translate (con_subst E e) b B buf_size) (translate t b B buf_size) else f t0) as threads''; remember (fun t0 => if thread_equals t0 thread then plus (translate (con_subst E e') b B buf_size) (translate t b B buf_size) else f t0) as threads'''. apply steps_app_right with (threads:=threads'') (threads':=threads''') (thread:=thread) (e2:=flush_star b B buf_size;; var "x") (x:="x").
+  + remember (fun t0 => if thread_equals t0 thread then plus (translate (con_subst E e) b B buf_size) (translate t b B buf_size) else f t0) as threads''; remember (fun t0 => if thread_equals t0 thread then plus (translate (con_subst E e') b B buf_size) (translate t b B buf_size) else f t0) as threads'''. apply steps_app_right with (threads:=threads'') (threads':=threads''') (thread:=thread) (e2:=flush_star b B buf_size;; var 0).
     ++ apply steps_plus_left with (threads:=threads) (threads':=threads') (thread:=thread) (e2:=translate t b B buf_size). apply IHE with (u:=u) (v:=v). rewrite Heqthreads'. auto. auto. rewrite Heqthreads. auto. auto. auto. rewrite Heqthreads''. rewrite Heqthreads. intros. destruct (thread_equals t0 thread). auto. auto. rewrite Heqthreads'''. rewrite Heqthreads'. intros. destruct (thread_equals t0 thread). auto. auto.
     ++ intros. destruct (thread_equals t0 thread) eqn:ORIG.
        +++ rewrite Heqthreads''. rewrite ORIG. rewrite H1. rewrite ORIG. auto.
@@ -430,7 +612,7 @@ Proof. intros. generalize dependent l. generalize dependent l'. generalize depen
     ++ intros. destruct (thread_equals t0 thread) eqn:ORIG.
        +++ rewrite Heqthreads'''. rewrite ORIG. rewrite H2. rewrite ORIG. auto.
        +++ rewrite Heqthreads'''. rewrite ORIG. rewrite H2. rewrite ORIG. auto.
-  + destruct s. destruct e0. subst x. rewrite translate_plus in *. rewrite translate_num in *. remember (fun t0 => if thread_equals t0 thread then plus (num x0) (translate (con_subst E e) b B buf_size) else f t0) as threads''; remember (fun t0 => if thread_equals t0 thread then plus (num x0) (translate (con_subst E e') b B buf_size)else f t0) as threads'''. apply steps_app_right with (threads:=threads'') (threads':=threads''') (thread:=thread) (e2:=flush_star b B buf_size;; var "x") (x:="x").
+  + destruct s. destruct e0. subst x. rewrite translate_plus in *. rewrite translate_num in *. remember (fun t0 => if thread_equals t0 thread then plus (num x0) (translate (con_subst E e) b B buf_size) else f t0) as threads''; remember (fun t0 => if thread_equals t0 thread then plus (num x0) (translate (con_subst E e') b B buf_size)else f t0) as threads'''. apply steps_app_right with (threads:=threads'') (threads':=threads''') (thread:=thread) (e2:=flush_star b B buf_size;; var 0).
     ++ apply steps_plus_right with (threads:=threads) (threads':=threads') (thread:=thread) (e2:=x0). apply IHE with (u:=u) (v:=v). rewrite Heqthreads'. auto. auto. rewrite Heqthreads. auto. auto. auto. rewrite Heqthreads''. rewrite Heqthreads. intros. destruct (thread_equals t thread). auto. auto. rewrite Heqthreads'''. rewrite Heqthreads'. intros. destruct (thread_equals t thread). auto. auto.
     ++ intros. destruct (thread_equals t thread) eqn:ORIG.
        +++ rewrite Heqthreads''. rewrite ORIG. rewrite H1. rewrite ORIG. auto.
@@ -438,7 +620,7 @@ Proof. intros. generalize dependent l. generalize dependent l'. generalize depen
     ++ intros. destruct (thread_equals t thread) eqn:ORIG.
        +++ rewrite Heqthreads'''. rewrite ORIG. rewrite H2. rewrite ORIG. auto.
        +++ rewrite Heqthreads'''. rewrite ORIG. rewrite H2. rewrite ORIG. auto.
-  + remember (fun t0 => if thread_equals t0 thread then minus (translate (con_subst E e) b B buf_size) (translate t b B buf_size) else f t0) as threads''; remember (fun t0 => if thread_equals t0 thread then minus (translate (con_subst E e') b B buf_size) (translate t b B buf_size) else f t0) as threads'''. apply steps_app_right with (threads:=threads'') (threads':=threads''') (thread:=thread) (e2:=flush_star b B buf_size;; var "x") (x:="x").
+  + remember (fun t0 => if thread_equals t0 thread then minus (translate (con_subst E e) b B buf_size) (translate t b B buf_size) else f t0) as threads''; remember (fun t0 => if thread_equals t0 thread then minus (translate (con_subst E e') b B buf_size) (translate t b B buf_size) else f t0) as threads'''. apply steps_app_right with (threads:=threads'') (threads':=threads''') (thread:=thread) (e2:=flush_star b B buf_size;; var 0).
     ++ apply steps_minus_left with (threads:=threads) (threads':=threads') (thread:=thread) (e2:=translate t b B buf_size). apply IHE with (u:=u) (v:=v). rewrite Heqthreads'. auto. auto. rewrite Heqthreads. auto. auto. auto. rewrite Heqthreads''. rewrite Heqthreads. intros. destruct (thread_equals t0 thread). auto. auto. rewrite Heqthreads'''. rewrite Heqthreads'. intros. destruct (thread_equals t0 thread). auto. auto.
     ++ intros. destruct (thread_equals t0 thread) eqn:ORIG.
        +++ rewrite Heqthreads''. rewrite ORIG. rewrite H1. rewrite ORIG. auto.
@@ -446,7 +628,7 @@ Proof. intros. generalize dependent l. generalize dependent l'. generalize depen
     ++ intros. destruct (thread_equals t0 thread) eqn:ORIG.
        +++ rewrite Heqthreads'''. rewrite ORIG. rewrite H2. rewrite ORIG. auto.
        +++ rewrite Heqthreads'''. rewrite ORIG. rewrite H2. rewrite ORIG. auto.
-  + destruct s. destruct e0. subst x. rewrite translate_minus in *. rewrite translate_num in *. remember (fun t0 => if thread_equals t0 thread then minus (num x0) (translate (con_subst E e) b B buf_size) else f t0) as threads''; remember (fun t0 => if thread_equals t0 thread then minus (num x0) (translate (con_subst E e') b B buf_size)else f t0) as threads'''. apply steps_app_right with (threads:=threads'') (threads':=threads''') (thread:=thread) (e2:=flush_star b B buf_size;; var "x") (x:="x").
+  + destruct s. destruct e0. subst x. rewrite translate_minus in *. rewrite translate_num in *. remember (fun t0 => if thread_equals t0 thread then minus (num x0) (translate (con_subst E e) b B buf_size) else f t0) as threads''; remember (fun t0 => if thread_equals t0 thread then minus (num x0) (translate (con_subst E e') b B buf_size)else f t0) as threads'''. apply steps_app_right with (threads:=threads'') (threads':=threads''') (thread:=thread) (e2:=flush_star b B buf_size;; var 0).
     ++ apply steps_minus_right with (threads:=threads) (threads':=threads') (thread:=thread) (e2:=x0). apply IHE with (u:=u) (v:=v). rewrite Heqthreads'. auto. auto. rewrite Heqthreads. auto. auto. auto. rewrite Heqthreads''. rewrite Heqthreads. intros. destruct (thread_equals t thread). auto. auto. rewrite Heqthreads'''. rewrite Heqthreads'. intros. destruct (thread_equals t thread). auto. auto.
     ++ intros. destruct (thread_equals t thread) eqn:ORIG.
        +++ rewrite Heqthreads''. rewrite ORIG. rewrite H1. rewrite ORIG. auto.
@@ -454,7 +636,7 @@ Proof. intros. generalize dependent l. generalize dependent l'. generalize depen
     ++ intros. destruct (thread_equals t thread) eqn:ORIG.
        +++ rewrite Heqthreads'''. rewrite ORIG. rewrite H2. rewrite ORIG. auto.
        +++ rewrite Heqthreads'''. rewrite ORIG. rewrite H2. rewrite ORIG. auto.
-  + remember (fun t0 => if thread_equals t0 thread then modulo (translate (con_subst E e) b B buf_size) (translate t b B buf_size) else f t0) as threads''; remember (fun t0 => if thread_equals t0 thread then modulo (translate (con_subst E e') b B buf_size) (translate t b B buf_size) else f t0) as threads'''. apply steps_app_right with (threads:=threads'') (threads':=threads''') (thread:=thread) (e2:=flush_star b B buf_size;; var "x") (x:="x").
+  + remember (fun t0 => if thread_equals t0 thread then modulo (translate (con_subst E e) b B buf_size) (translate t b B buf_size) else f t0) as threads''; remember (fun t0 => if thread_equals t0 thread then modulo (translate (con_subst E e') b B buf_size) (translate t b B buf_size) else f t0) as threads'''. apply steps_app_right with (threads:=threads'') (threads':=threads''') (thread:=thread) (e2:=flush_star b B buf_size;; var 0).
     ++ apply steps_modulo_left with (threads:=threads) (threads':=threads') (thread:=thread) (e2:=translate t b B buf_size). apply IHE with (u:=u) (v:=v). rewrite Heqthreads'. auto. auto. rewrite Heqthreads. auto. auto. auto. rewrite Heqthreads''. rewrite Heqthreads. intros. destruct (thread_equals t0 thread). auto. auto. rewrite Heqthreads'''. rewrite Heqthreads'. intros. destruct (thread_equals t0 thread). auto. auto.
     ++ intros. destruct (thread_equals t0 thread) eqn:ORIG.
        +++ rewrite Heqthreads''. rewrite ORIG. rewrite H1. rewrite ORIG. auto.
@@ -462,7 +644,7 @@ Proof. intros. generalize dependent l. generalize dependent l'. generalize depen
     ++ intros. destruct (thread_equals t0 thread) eqn:ORIG.
        +++ rewrite Heqthreads'''. rewrite ORIG. rewrite H2. rewrite ORIG. auto.
        +++ rewrite Heqthreads'''. rewrite ORIG. rewrite H2. rewrite ORIG. auto.
-  + destruct s. destruct e0. subst x. rewrite translate_modulo in *. rewrite translate_num in *. remember (fun t0 => if thread_equals t0 thread then modulo (num x0) (translate (con_subst E e) b B buf_size) else f t0) as threads''; remember (fun t0 => if thread_equals t0 thread then modulo (num x0) (translate (con_subst E e') b B buf_size)else f t0) as threads'''. apply steps_app_right with (threads:=threads'') (threads':=threads''') (thread:=thread) (e2:=flush_star b B buf_size;; var "x") (x:="x").
+  + destruct s. destruct e0. subst x. rewrite translate_modulo in *. rewrite translate_num in *. remember (fun t0 => if thread_equals t0 thread then modulo (num x0) (translate (con_subst E e) b B buf_size) else f t0) as threads''; remember (fun t0 => if thread_equals t0 thread then modulo (num x0) (translate (con_subst E e') b B buf_size)else f t0) as threads'''. apply steps_app_right with (threads:=threads'') (threads':=threads''') (thread:=thread) (e2:=flush_star b B buf_size;; var 0).
     ++ apply steps_modulo_right with (threads:=threads) (threads':=threads') (thread:=thread) (e2:=x0). apply IHE with (u:=u) (v:=v). rewrite Heqthreads'. auto. auto. rewrite Heqthreads. auto. auto. auto. rewrite Heqthreads''. rewrite Heqthreads. intros. destruct (thread_equals t thread). auto. auto. rewrite Heqthreads'''. rewrite Heqthreads'. intros. destruct (thread_equals t thread). auto. auto.
     ++ intros. destruct (thread_equals t thread) eqn:ORIG.
        +++ rewrite Heqthreads''. rewrite ORIG. rewrite H1. rewrite ORIG. auto.
@@ -470,7 +652,7 @@ Proof. intros. generalize dependent l. generalize dependent l'. generalize depen
     ++ intros. destruct (thread_equals t thread) eqn:ORIG.
        +++ rewrite Heqthreads'''. rewrite ORIG. rewrite H2. rewrite ORIG. auto.
        +++ rewrite Heqthreads'''. rewrite ORIG. rewrite H2. rewrite ORIG. auto.
-  + remember (fun t0 => if thread_equals t0 thread then less_than (translate (con_subst E e) b B buf_size) (translate t b B buf_size) else f t0) as threads''; remember (fun t0 => if thread_equals t0 thread then less_than (translate (con_subst E e') b B buf_size) (translate t b B buf_size) else f t0) as threads'''. apply steps_app_right with (threads:=threads'') (threads':=threads''') (thread:=thread) (e2:=flush_star b B buf_size;; var "x") (x:="x").
+  + remember (fun t0 => if thread_equals t0 thread then less_than (translate (con_subst E e) b B buf_size) (translate t b B buf_size) else f t0) as threads''; remember (fun t0 => if thread_equals t0 thread then less_than (translate (con_subst E e') b B buf_size) (translate t b B buf_size) else f t0) as threads'''. apply steps_app_right with (threads:=threads'') (threads':=threads''') (thread:=thread) (e2:=flush_star b B buf_size;; var 0).
     ++ apply steps_less_than_left with (threads:=threads) (threads':=threads') (thread:=thread) (e2:=translate t b B buf_size). apply IHE with (u:=u) (v:=v). rewrite Heqthreads'. auto. auto. rewrite Heqthreads. auto. auto. auto. rewrite Heqthreads''. rewrite Heqthreads. intros. destruct (thread_equals t0 thread). auto. auto. rewrite Heqthreads'''. rewrite Heqthreads'. intros. destruct (thread_equals t0 thread). auto. auto.
     ++ intros. destruct (thread_equals t0 thread) eqn:ORIG.
        +++ rewrite Heqthreads''. rewrite ORIG. rewrite H1. rewrite ORIG. auto.
@@ -478,7 +660,7 @@ Proof. intros. generalize dependent l. generalize dependent l'. generalize depen
     ++ intros. destruct (thread_equals t0 thread) eqn:ORIG.
        +++ rewrite Heqthreads'''. rewrite ORIG. rewrite H2. rewrite ORIG. auto.
        +++ rewrite Heqthreads'''. rewrite ORIG. rewrite H2. rewrite ORIG. auto.
-  + destruct s. destruct e0. subst x. rewrite translate_less_than in *. rewrite translate_num in *. remember (fun t0 => if thread_equals t0 thread then less_than (num x0) (translate (con_subst E e) b B buf_size) else f t0) as threads''; remember (fun t0 => if thread_equals t0 thread then less_than (num x0) (translate (con_subst E e') b B buf_size)else f t0) as threads'''. apply steps_app_right with (threads:=threads'') (threads':=threads''') (thread:=thread) (e2:=flush_star b B buf_size;; var "x") (x:="x").
+  + destruct s. destruct e0. subst x. rewrite translate_less_than in *. rewrite translate_num in *. remember (fun t0 => if thread_equals t0 thread then less_than (num x0) (translate (con_subst E e) b B buf_size) else f t0) as threads''; remember (fun t0 => if thread_equals t0 thread then less_than (num x0) (translate (con_subst E e') b B buf_size)else f t0) as threads'''. apply steps_app_right with (threads:=threads'') (threads':=threads''') (thread:=thread) (e2:=flush_star b B buf_size;; var 0).
     ++ apply steps_less_than_right with (threads:=threads) (threads':=threads') (thread:=thread) (e2:=x0). apply IHE with (u:=u) (v:=v). rewrite Heqthreads'. auto. auto. rewrite Heqthreads. auto. auto. auto. rewrite Heqthreads''. rewrite Heqthreads. intros. destruct (thread_equals t thread). auto. auto. rewrite Heqthreads'''. rewrite Heqthreads'. intros. destruct (thread_equals t thread). auto. auto.
     ++ intros. destruct (thread_equals t thread) eqn:ORIG.
        +++ rewrite Heqthreads''. rewrite ORIG. rewrite H1. rewrite ORIG. auto.
@@ -486,7 +668,7 @@ Proof. intros. generalize dependent l. generalize dependent l'. generalize depen
     ++ intros. destruct (thread_equals t thread) eqn:ORIG.
        +++ rewrite Heqthreads'''. rewrite ORIG. rewrite H2. rewrite ORIG. auto.
        +++ rewrite Heqthreads'''. rewrite ORIG. rewrite H2. rewrite ORIG. auto.
-  + remember (fun t0 => if thread_equals t0 thread then and (translate (con_subst E e) b B buf_size) (translate t b B buf_size) else f t0) as threads''; remember (fun t0 => if thread_equals t0 thread then and (translate (con_subst E e') b B buf_size) (translate t b B buf_size) else f t0) as threads'''. apply steps_app_right with (threads:=threads'') (threads':=threads''') (thread:=thread) (e2:=flush_star b B buf_size;; var "x") (x:="x").
+  + remember (fun t0 => if thread_equals t0 thread then and (translate (con_subst E e) b B buf_size) (translate t b B buf_size) else f t0) as threads''; remember (fun t0 => if thread_equals t0 thread then and (translate (con_subst E e') b B buf_size) (translate t b B buf_size) else f t0) as threads'''. apply steps_app_right with (threads:=threads'') (threads':=threads''') (thread:=thread) (e2:=flush_star b B buf_size;; var 0).
     ++ apply steps_and_left with (threads:=threads) (threads':=threads') (thread:=thread) (e2:=translate t b B buf_size). apply IHE with (u:=u) (v:=v). rewrite Heqthreads'. auto. auto. rewrite Heqthreads. auto. auto. auto. rewrite Heqthreads''. rewrite Heqthreads. intros. destruct (thread_equals t0 thread). auto. auto. rewrite Heqthreads'''. rewrite Heqthreads'. intros. destruct (thread_equals t0 thread). auto. auto.
     ++ intros. destruct (thread_equals t0 thread) eqn:ORIG.
        +++ rewrite Heqthreads''. rewrite ORIG. rewrite H1. rewrite ORIG. auto.
@@ -494,7 +676,7 @@ Proof. intros. generalize dependent l. generalize dependent l'. generalize depen
     ++ intros. destruct (thread_equals t0 thread) eqn:ORIG.
        +++ rewrite Heqthreads'''. rewrite ORIG. rewrite H2. rewrite ORIG. auto.
        +++ rewrite Heqthreads'''. rewrite ORIG. rewrite H2. rewrite ORIG. auto.
-  + destruct s. subst x. rewrite translate_and in *. rewrite translate_tru in *. remember (fun t0 => if thread_equals t0 thread then and tru (translate (con_subst E e) b B buf_size) else f t0) as threads''; remember (fun t0 => if thread_equals t0 thread then and tru (translate (con_subst E e')  b B buf_size) else f t0) as threads'''. apply steps_app_right with (threads:=threads'') (threads':=threads''') (thread:=thread) (e2:=flush_star b B buf_size;; var "x") (x:="x").
+  + destruct s. subst x. rewrite translate_and in *. rewrite translate_tru in *. remember (fun t0 => if thread_equals t0 thread then and tru (translate (con_subst E e) b B buf_size) else f t0) as threads''; remember (fun t0 => if thread_equals t0 thread then and tru (translate (con_subst E e')  b B buf_size) else f t0) as threads'''. apply steps_app_right with (threads:=threads'') (threads':=threads''') (thread:=thread) (e2:=flush_star b B buf_size;; var 0).
     ++ apply steps_and_right with (threads:=threads) (threads':=threads') (thread:=thread). apply IHE with (u:=u) (v:=v). rewrite Heqthreads'. auto. auto. rewrite Heqthreads. auto. auto. auto. rewrite Heqthreads''. rewrite Heqthreads. intros. destruct (thread_equals t thread). auto. auto. rewrite Heqthreads'''. rewrite Heqthreads'. intros. destruct (thread_equals t thread). auto. auto.
     ++ intros. destruct (thread_equals t thread) eqn:ORIG.
        +++ rewrite Heqthreads''. rewrite ORIG. rewrite H1. rewrite ORIG. auto.
@@ -502,34 +684,34 @@ Proof. intros. generalize dependent l. generalize dependent l'. generalize depen
     ++ intros. destruct (thread_equals t thread) eqn:ORIG.
        +++ rewrite Heqthreads'''. rewrite ORIG. rewrite H2. rewrite ORIG. auto.
        +++ rewrite Heqthreads'''. rewrite ORIG. rewrite H2. rewrite ORIG. auto.
-  + unfold new_read in *. remember (fun t0 => if thread_equals t0 thread then app (lam "pair" (read_code b B buf_size))  (paire (translate (con_subst E e) b B buf_size) (translate t b B buf_size)) else f t0) as threads''. remember (fun t0 => if thread_equals t0 thread then app (lam "pair" (read_code b B buf_size))  (paire (translate (con_subst E e') b B buf_size) (translate t b B buf_size)) else f t0) as threads'''. apply steps_app_right with (threads:=threads'') (threads':=threads''') (thread:=thread) (e2:=flush_star b B buf_size;; var "x") (x:="x").
-    ++ remember (fun t0 => if thread_equals t0 thread then (paire (translate (con_subst E e) b B buf_size) (translate t b B buf_size)) else f t0) as threads''''. remember (fun t0 => if thread_equals t0 thread then (paire (translate (con_subst E e') b B buf_size) (translate t b B buf_size)) else f t0) as threads'''''. apply steps_app_right with (threads:=threads'''') (threads':=threads''''') (thread:=thread) (e2:=read_code b B buf_size) (x:="pair").
+  + unfold new_read in *. remember (fun t0 => if thread_equals t0 thread then app (lam (read_code b B buf_size))  (paire (translate (con_subst E e) b B buf_size) (translate t b B buf_size)) else f t0) as threads''. remember (fun t0 => if thread_equals t0 thread then app (lam (read_code b B buf_size))  (paire (translate (con_subst E e') b B buf_size) (translate t b B buf_size)) else f t0) as threads'''. apply steps_app_right with (threads:=threads'') (threads':=threads''') (thread:=thread) (e2:=flush_star b B buf_size;; var 0).
+    ++ remember (fun t0 => if thread_equals t0 thread then (paire (translate (con_subst E e) b B buf_size) (translate t b B buf_size)) else f t0) as threads''''. remember (fun t0 => if thread_equals t0 thread then (paire (translate (con_subst E e') b B buf_size) (translate t b B buf_size)) else f t0) as threads'''''. apply steps_app_right with (threads:=threads'''') (threads':=threads''''') (thread:=thread) (e2:=read_code b B buf_size).
        +++ apply steps_paire_left with (threads:=threads) (threads':=threads') (thread:=thread) (e2:=translate t b B buf_size). apply IHE with (u:=u) (v:=v). rewrite Heqthreads'. auto. auto. rewrite Heqthreads. auto. auto. auto. rewrite Heqthreads''''. rewrite Heqthreads. intros. destruct (thread_equals t0 thread). auto. auto. rewrite Heqthreads'''''. rewrite Heqthreads'. intros. destruct (thread_equals t0 thread). auto. auto.
        +++ rewrite Heqthreads''''. rewrite Heqthreads''. intros. destruct (thread_equals t0 thread). auto. auto.
        +++ rewrite Heqthreads'''''. rewrite Heqthreads'''. intros. destruct (thread_equals t0 thread). auto. auto.
     ++ intros. rewrite H1. rewrite Heqthreads''. destruct (thread_equals t0 thread). auto. auto.
     ++ intros. rewrite H2. rewrite Heqthreads'''. destruct (thread_equals t0 thread). auto. auto.
-  + destruct s. destruct e0. subst x. rewrite translate_read in *. unfold new_read in *. rewrite translate_array in *. remember (fun t0 => if thread_equals t0 thread then app (lam "pair" (read_code b B buf_size))  (paire (array x0) (translate (con_subst E e) b B buf_size) ) else f t0) as threads''. remember (fun t0 => if thread_equals t0 thread then app (lam "pair" (read_code b B buf_size))  (paire (array x0) (translate (con_subst E e') b B buf_size)) else f t0) as threads'''. apply steps_app_right with (threads:=threads'') (threads':=threads''') (thread:=thread) (e2:=flush_star b B buf_size;; var "x") (x:="x").
-    ++ remember (fun t0 => if thread_equals t0 thread then (paire (array x0) (translate (con_subst E e) b B buf_size)) else f t0) as threads''''. remember (fun t0 => if thread_equals t0 thread then (paire (array x0) (translate (con_subst E e') b B buf_size)) else f t0) as threads'''''. apply steps_app_right with (threads:=threads'''') (threads':=threads''''') (thread:=thread) (e2:=read_code b B buf_size) (x:="pair").
+  + destruct s. destruct e0. subst x. rewrite translate_read in *. unfold new_read in *. rewrite translate_array in *. remember (fun t0 => if thread_equals t0 thread then app (lam (read_code b B buf_size))  (paire (array x0) (translate (con_subst E e) b B buf_size) ) else f t0) as threads''. remember (fun t0 => if thread_equals t0 thread then app (lam (read_code b B buf_size))  (paire (array x0) (translate (con_subst E e') b B buf_size)) else f t0) as threads'''. apply steps_app_right with (threads:=threads'') (threads':=threads''') (thread:=thread) (e2:=flush_star b B buf_size;; var 0).
+    ++ remember (fun t0 => if thread_equals t0 thread then (paire (array x0) (translate (con_subst E e) b B buf_size)) else f t0) as threads''''. remember (fun t0 => if thread_equals t0 thread then (paire (array x0) (translate (con_subst E e') b B buf_size)) else f t0) as threads'''''. apply steps_app_right with (threads:=threads'''') (threads':=threads''''') (thread:=thread) (e2:=read_code b B buf_size).
        +++ apply steps_paire_right with (threads:=threads) (threads':=threads') (thread:=thread) (e2:=array x0). apply IHE with (u:=u) (v:=v). rewrite Heqthreads'. auto. auto. rewrite Heqthreads. auto. auto. auto. apply value_array. rewrite Heqthreads''''. rewrite Heqthreads. intros. destruct (thread_equals t thread). auto. auto. rewrite Heqthreads'''''. rewrite Heqthreads'. intros. destruct (thread_equals t thread). auto. auto.
        +++ rewrite Heqthreads''''. rewrite Heqthreads''. intros. destruct (thread_equals t thread). auto. auto.
        +++ rewrite Heqthreads'''''. rewrite Heqthreads'''. intros. destruct (thread_equals t thread). auto. auto.
     ++ intros. rewrite H1. rewrite Heqthreads''. destruct (thread_equals t thread). auto. auto.
     ++ intros. rewrite H2. rewrite Heqthreads'''. destruct (thread_equals t thread). auto. auto.
-  + unfold new_write in *. remember (fun q => if thread_equals q thread then app (lam "triple" (write_code b B buf_size)) (paire (translate (con_subst E e) b B buf_size) (paire (translate t b B buf_size) (translate t0 b B buf_size))) else f q) as threads''. remember (fun q => if thread_equals q thread then app (lam "triple" (write_code b B buf_size)) (paire (translate (con_subst E e') b B buf_size) (paire (translate t b B buf_size) (translate t0 b B buf_size))) else f q) as threads'''. apply steps_app_right with (threads:=threads'') (threads':=threads''') (thread:=thread) (e2:=flush_star b B buf_size;; var "x") (x:="x").
+  + unfold new_write in *. remember (fun q => if thread_equals q thread then app (lam (write_code b B buf_size)) (paire (translate (con_subst E e) b B buf_size) (paire (translate t b B buf_size) (translate t0 b B buf_size))) else f q) as threads''. remember (fun q => if thread_equals q thread then app (lam (write_code b B buf_size)) (paire (translate (con_subst E e') b B buf_size) (paire (translate t b B buf_size) (translate t0 b B buf_size))) else f q) as threads'''. apply steps_app_right with (threads:=threads'') (threads':=threads''') (thread:=thread) (e2:=flush_star b B buf_size;; var 0).
     ++ remember (fun q => if thread_equals q thread then paire (translate (con_subst E e) b B buf_size)
-                        (paire (translate t b B buf_size) (translate t0 b B buf_size)) else f q) as threads''''. remember (fun q => if thread_equals q thread then paire (translate (con_subst E e') b B buf_size) (paire (translate t b B buf_size) (translate t0 b B buf_size)) else f q) as threads'''''. apply steps_app_right with (threads:=threads'''') (threads':=threads''''') (thread:=thread) (e2:=write_code b B buf_size) (x:="triple").
+                        (paire (translate t b B buf_size) (translate t0 b B buf_size)) else f q) as threads''''. remember (fun q => if thread_equals q thread then paire (translate (con_subst E e') b B buf_size) (paire (translate t b B buf_size) (translate t0 b B buf_size)) else f q) as threads'''''. apply steps_app_right with (threads:=threads'''') (threads':=threads''''') (thread:=thread) (e2:=write_code b B buf_size).
        +++ apply steps_paire_left with (threads:=threads) (threads':=threads') (thread:=thread) (e2:=paire (translate t b B buf_size) (translate t0 b B buf_size)). apply IHE with (u:=u) (v:=v). rewrite Heqthreads'. auto. auto. rewrite Heqthreads. auto. auto. auto. rewrite Heqthreads''''. rewrite Heqthreads. intros. destruct (thread_equals t1 thread) eqn:ORIG. auto. auto. rewrite Heqthreads'''''. intros. destruct (thread_equals t1 thread) eqn:ORIG. rewrite Heqthreads'. rewrite ORIG. auto. rewrite Heqthreads'. rewrite ORIG. auto.
        +++ rewrite Heqthreads''''. intros. rewrite Heqthreads''. destruct (thread_equals t1 thread) eqn:ORIG. auto. auto.
        +++ rewrite Heqthreads'''''. rewrite Heqthreads'''. intros. destruct (thread_equals t1 thread). auto. auto.
     ++ intros. rewrite H1. rewrite Heqthreads''. destruct (thread_equals t1 thread). auto. auto.
     ++ intros. rewrite H2. rewrite Heqthreads'''. destruct (thread_equals t1 thread). auto. auto.
-  + destruct s. destruct e0. subst x. rewrite translate_write in *. unfold new_write in *. rewrite translate_array in *. remember (fun q => if thread_equals q thread then app (lam "triple" (write_code b B buf_size)) (paire (array x0) (paire (translate (con_subst E e) b B buf_size) (translate t b B buf_size))) else f q) as threads''. remember (fun q => if thread_equals q thread then app (lam "triple" (write_code b B buf_size)) (paire (array x0) (paire (translate (con_subst E e') b B buf_size) (translate t b B buf_size))) else f q) as threads'''. apply steps_app_right with (threads:=threads'') (threads':=threads''') (thread:=thread) (e2:=flush_star b B buf_size;; var "x") (x:="x").
+  + destruct s. destruct e0. subst x. rewrite translate_write in *. unfold new_write in *. rewrite translate_array in *. remember (fun q => if thread_equals q thread then app (lam (write_code b B buf_size)) (paire (array x0) (paire (translate (con_subst E e) b B buf_size) (translate t b B buf_size))) else f q) as threads''. remember (fun q => if thread_equals q thread then app (lam (write_code b B buf_size)) (paire (array x0) (paire (translate (con_subst E e') b B buf_size) (translate t b B buf_size))) else f q) as threads'''. apply steps_app_right with (threads:=threads'') (threads':=threads''') (thread:=thread) (e2:=flush_star b B buf_size;; var 0).
     ++ remember (fun q => if thread_equals q thread then (paire (array x0)
                         (paire (translate (con_subst E e) b B buf_size)
                            (translate t b B buf_size))) else f q) as threads''''. remember (fun q => if thread_equals q thread then (paire (array x0)
                         (paire (translate (con_subst E e') b B buf_size)
-                           (translate t b B buf_size))) else f q) as threads'''''. apply steps_app_right with (threads:=threads'''') (threads':=threads''''') (thread:=thread) (e2:=write_code b B buf_size) (x:="triple").
+                           (translate t b B buf_size))) else f q) as threads'''''. apply steps_app_right with (threads:=threads'''') (threads':=threads''''') (thread:=thread) (e2:=write_code b B buf_size).
        +++ remember (fun q => if thread_equals q thread then (
                         (paire (translate (con_subst E e) b B buf_size)
                            (translate t b B buf_size))) else f q) as threads''''''. remember (fun q => if thread_equals q thread then (
@@ -543,10 +725,10 @@ Proof. intros. generalize dependent l. generalize dependent l'. generalize depen
        +++ rewrite Heqthreads'''. rewrite Heqthreads'''''. intros. destruct (thread_equals t0 thread). auto. auto.
     ++ intros. rewrite H1. rewrite Heqthreads''. destruct (thread_equals t0 thread). auto. auto.
     ++ intros. rewrite H2. rewrite Heqthreads'''. destruct (thread_equals t0 thread). auto. auto.
-  + destruct s. destruct e0. destruct s0. destruct e0. subst x. subst x1. rewrite translate_write in *. unfold new_write in *. rewrite translate_array in *. rewrite translate_num in *. remember (fun q => if thread_equals q thread then app (lam "triple" (write_code b B buf_size)) (paire (array x0) (paire (num x2) (translate (con_subst E e) b B buf_size))) else f q) as threads''. remember (fun q => if thread_equals q thread then app (lam "triple" (write_code b B buf_size)) (paire (array x0) (paire (num x2) (translate (con_subst E e') b B buf_size))) else f q) as threads'''. apply steps_app_right with (threads:=threads'') (threads':=threads''') (thread:=thread) (e2:=flush_star b B buf_size;; var "x") (x:="x").
+  + destruct s. destruct e0. destruct s0. destruct e0. subst x. subst x1. rewrite translate_write in *. unfold new_write in *. rewrite translate_array in *. rewrite translate_num in *. remember (fun q => if thread_equals q thread then app (lam (write_code b B buf_size)) (paire (array x0) (paire (num x2) (translate (con_subst E e) b B buf_size))) else f q) as threads''. remember (fun q => if thread_equals q thread then app (lam (write_code b B buf_size)) (paire (array x0) (paire (num x2) (translate (con_subst E e') b B buf_size))) else f q) as threads'''. apply steps_app_right with (threads:=threads'') (threads':=threads''') (thread:=thread) (e2:=flush_star b B buf_size;; var 0).
     ++ remember (fun q => if thread_equals q thread then (paire (array x0)
                         (paire (num x2) (translate (con_subst E e) b B buf_size))) else f q) as threads''''. remember (fun q => if thread_equals q thread then (paire (array x0)
-                        (paire (num x2) (translate (con_subst E e') b B buf_size))) else f q) as threads'''''. apply steps_app_right with (threads:=threads'''') (threads':=threads''''') (thread:=thread) (e2:=write_code b B buf_size) (x:="triple").
+                        (paire (num x2) (translate (con_subst E e') b B buf_size))) else f q) as threads'''''. apply steps_app_right with (threads:=threads'''') (threads':=threads''''') (thread:=thread) (e2:=write_code b B buf_size).
        +++ remember (fun q => if thread_equals q thread then (
                         (paire (num x2) (translate (con_subst E e) b B buf_size))) else f q) as threads''''''. remember (fun q => if thread_equals q thread then (
                         (paire (num x2) (translate (con_subst E e') b B buf_size))) else f q) as threads'''''''. apply steps_paire_right with (threads:=threads'''''') (threads':=threads''''''') (thread:=thread) (e2:=array x0).
@@ -564,7 +746,7 @@ Proof. intros. generalize dependent l. generalize dependent l'. generalize depen
        +++ intros. destruct (thread_equals t1 thread) eqn:ORIG.
            ++++ rewrite Heqthreads'. rewrite ORIG. rewrite H2. rewrite ORIG. auto.
            ++++ rewrite Heqthreads'. rewrite ORIG. rewrite H2. rewrite ORIG. auto.
-  + remember (fun t0 => if thread_equals t0 thread then not (translate (con_subst E e) b B buf_size) else f t0) as threads''; remember (fun t0 => if thread_equals t0 thread then not (translate (con_subst E e') b B buf_size)else f t0) as threads'''. apply steps_app_right with (threads:=threads'') (threads':=threads''') (thread:=thread) (e2:=flush_star b B buf_size;; var "x") (x:="x").
+  + remember (fun t0 => if thread_equals t0 thread then not (translate (con_subst E e) b B buf_size) else f t0) as threads''; remember (fun t0 => if thread_equals t0 thread then not (translate (con_subst E e') b B buf_size)else f t0) as threads'''. apply steps_app_right with (threads:=threads'') (threads':=threads''') (thread:=thread) (e2:=flush_star b B buf_size;; var 0).
     ++ apply steps_not_left with (threads:=threads) (threads':=threads') (thread:=thread). apply IHE with (u:=u) (v:=v). rewrite Heqthreads'. auto. auto. rewrite Heqthreads. auto. auto. auto. rewrite Heqthreads''. rewrite Heqthreads. intros. destruct (thread_equals t thread). auto. auto. rewrite Heqthreads'''. rewrite Heqthreads'. intros. destruct (thread_equals t thread). auto. auto.
     ++ intros. destruct (thread_equals t thread) eqn:ORIG.
        +++ rewrite Heqthreads''. rewrite ORIG. rewrite H1. rewrite ORIG. auto.
@@ -572,7 +754,7 @@ Proof. intros. generalize dependent l. generalize dependent l'. generalize depen
     ++ intros. destruct (thread_equals t thread) eqn:ORIG.
        +++ rewrite Heqthreads'''. rewrite ORIG. rewrite H2. rewrite ORIG. auto.
        +++ rewrite Heqthreads'''. rewrite ORIG. rewrite H2. rewrite ORIG. auto.
-  + remember (fun t0 => if thread_equals t0 thread then reference (translate (con_subst E e) b B buf_size) else f t0) as threads''; remember (fun t0 => if thread_equals t0 thread then reference (translate (con_subst E e') b B buf_size)else f t0) as threads'''. apply steps_app_right with (threads:=threads'') (threads':=threads''') (thread:=thread) (e2:=flush_star b B buf_size;; var "x") (x:="x").
+  + remember (fun t0 => if thread_equals t0 thread then reference (translate (con_subst E e) b B buf_size) else f t0) as threads''; remember (fun t0 => if thread_equals t0 thread then reference (translate (con_subst E e') b B buf_size)else f t0) as threads'''. apply steps_app_right with (threads:=threads'') (threads':=threads''') (thread:=thread) (e2:=flush_star b B buf_size;; var 0).
     ++ apply steps_reference_left with (threads:=threads) (threads':=threads') (thread:=thread). apply IHE with (u:=u) (v:=v). rewrite Heqthreads'. auto. auto. rewrite Heqthreads. auto. auto. auto. rewrite Heqthreads''. rewrite Heqthreads. intros. destruct (thread_equals t thread). auto. auto. rewrite Heqthreads'''. rewrite Heqthreads'. intros. destruct (thread_equals t thread). auto. auto.
     ++ intros. destruct (thread_equals t thread) eqn:ORIG.
        +++ rewrite Heqthreads''. rewrite ORIG. rewrite H1. rewrite ORIG. auto.
@@ -580,7 +762,7 @@ Proof. intros. generalize dependent l. generalize dependent l'. generalize depen
     ++ intros. destruct (thread_equals t thread) eqn:ORIG.
        +++ rewrite Heqthreads'''. rewrite ORIG. rewrite H2. rewrite ORIG. auto.
        +++ rewrite Heqthreads'''. rewrite ORIG. rewrite H2. rewrite ORIG. auto.
-  + remember (fun t0 => if thread_equals t0 thread then cast (translate (con_subst E e) b B buf_size) else f t0) as threads''; remember (fun t0 => if thread_equals t0 thread then cast (translate (con_subst E e') b B buf_size)else f t0) as threads'''. apply steps_app_right with (threads:=threads'') (threads':=threads''') (thread:=thread) (e2:=flush_star b B buf_size;; var "x") (x:="x").
+  + remember (fun t0 => if thread_equals t0 thread then cast (translate (con_subst E e) b B buf_size) else f t0) as threads''; remember (fun t0 => if thread_equals t0 thread then cast (translate (con_subst E e') b B buf_size)else f t0) as threads'''. apply steps_app_right with (threads:=threads'') (threads':=threads''') (thread:=thread) (e2:=flush_star b B buf_size;; var 0).
     ++ apply steps_cast_left with (threads:=threads) (threads':=threads') (thread:=thread). apply IHE with (u:=u) (v:=v). rewrite Heqthreads'. auto. auto. rewrite Heqthreads. auto. auto. auto. rewrite Heqthreads''. rewrite Heqthreads. intros. destruct (thread_equals t thread). auto. auto. rewrite Heqthreads'''. rewrite Heqthreads'. intros. destruct (thread_equals t thread). auto. auto.
     ++ intros. destruct (thread_equals t thread) eqn:ORIG.
        +++ rewrite Heqthreads''. rewrite ORIG. rewrite H1. rewrite ORIG. auto.
@@ -590,7 +772,7 @@ Proof. intros. generalize dependent l. generalize dependent l'. generalize depen
        +++ rewrite Heqthreads'''. rewrite ORIG. rewrite H2. rewrite ORIG. auto.
   + apply steps_paire_left with (threads:=threads) (threads':=threads') (thread:=thread) (e2:=translate t b B buf_size). apply IHE with (u:=u) (v:=v). rewrite Heqthreads'. auto. auto. rewrite Heqthreads. intros. destruct (thread_equals t0 thread) eqn:ORIG. auto. auto. intros. rewrite H. auto. auto. intros. rewrite H1. destruct (thread_equals t0 thread) eqn:ORIG. rewrite Heqthreads. rewrite ORIG. auto. rewrite Heqthreads. rewrite ORIG. auto. intros. destruct (thread_equals t0 thread) eqn:ORIG. rewrite H2. rewrite ORIG. rewrite Heqthreads'. rewrite ORIG. auto. rewrite Heqthreads'. rewrite ORIG. rewrite H2. rewrite ORIG. auto.
   + destruct s. apply steps_paire_right with (threads:=threads) (threads':=threads') (thread:=thread) (e2:=translate x b B buf_size). apply IHE with (u:=u) (v:=v). rewrite Heqthreads'. auto. auto. rewrite Heqthreads. intros. auto. intros. rewrite H. auto. auto. apply translation_of_value_is_value. auto. intros. destruct (thread_equals t thread) eqn:ORIG. rewrite H1. rewrite ORIG. rewrite Heqthreads. rewrite ORIG. rewrite translate_paire. auto. rewrite Heqthreads. rewrite ORIG. rewrite H1. rewrite ORIG. auto. intros. destruct (thread_equals t thread) eqn:ORIG. rewrite H2. rewrite ORIG. rewrite Heqthreads'. rewrite ORIG. rewrite translate_paire. auto. rewrite Heqthreads'. rewrite ORIG. rewrite H2. rewrite ORIG. auto.
-  + remember (fun t0 => if thread_equals t0 thread then first (translate (con_subst E e) b B buf_size) else f t0) as threads''; remember (fun t0 => if thread_equals t0 thread then first (translate (con_subst E e') b B buf_size)else f t0) as threads'''. apply steps_app_right with (threads:=threads'') (threads':=threads''') (thread:=thread) (e2:=flush_star b B buf_size;; var "x") (x:="x").
+  + remember (fun t0 => if thread_equals t0 thread then first (translate (con_subst E e) b B buf_size) else f t0) as threads''; remember (fun t0 => if thread_equals t0 thread then first (translate (con_subst E e') b B buf_size)else f t0) as threads'''. apply steps_app_right with (threads:=threads'') (threads':=threads''') (thread:=thread) (e2:=flush_star b B buf_size;; var 0).
     ++ apply steps_first_left with (threads:=threads) (threads':=threads') (thread:=thread). apply IHE with (u:=u) (v:=v). rewrite Heqthreads'. auto. auto. rewrite Heqthreads. auto. auto. auto. rewrite Heqthreads''. rewrite Heqthreads. intros. destruct (thread_equals t thread). auto. auto. rewrite Heqthreads'''. rewrite Heqthreads'. intros. destruct (thread_equals t thread). auto. auto.
     ++ intros. destruct (thread_equals t thread) eqn:ORIG.
        +++ rewrite Heqthreads''. rewrite ORIG. rewrite H1. rewrite ORIG. auto.
@@ -598,7 +780,7 @@ Proof. intros. generalize dependent l. generalize dependent l'. generalize depen
     ++ intros. destruct (thread_equals t thread) eqn:ORIG.
        +++ rewrite Heqthreads'''. rewrite ORIG. rewrite H2. rewrite ORIG. auto.
        +++ rewrite Heqthreads'''. rewrite ORIG. rewrite H2. rewrite ORIG. auto.
-  + remember (fun t0 => if thread_equals t0 thread then second (translate (con_subst E e) b B buf_size) else f t0) as threads''; remember (fun t0 => if thread_equals t0 thread then second (translate (con_subst E e') b B buf_size)else f t0) as threads'''. apply steps_app_right with (threads:=threads'') (threads':=threads''') (thread:=thread) (e2:=flush_star b B buf_size;; var "x") (x:="x").
+  + remember (fun t0 => if thread_equals t0 thread then second (translate (con_subst E e) b B buf_size) else f t0) as threads''; remember (fun t0 => if thread_equals t0 thread then second (translate (con_subst E e') b B buf_size)else f t0) as threads'''. apply steps_app_right with (threads:=threads'') (threads':=threads''') (thread:=thread) (e2:=flush_star b B buf_size;; var 0).
     ++ apply steps_second_left with (threads:=threads) (threads':=threads') (thread:=thread). apply IHE with (u:=u) (v:=v). rewrite Heqthreads'. auto. auto. rewrite Heqthreads. auto. auto. auto. rewrite Heqthreads''. rewrite Heqthreads. intros. destruct (thread_equals t thread). auto. auto. rewrite Heqthreads'''. rewrite Heqthreads'. intros. destruct (thread_equals t thread). auto. auto.
     ++ intros. destruct (thread_equals t thread) eqn:ORIG.
        +++ rewrite Heqthreads''. rewrite ORIG. rewrite H1. rewrite ORIG. auto.
